Strengthen statement and prove Let case

compiler/backend/bvi_to_dataScript.sml
@@ -130,9 +130,10 @@ Definition compile_def:
          (Seq c1 (If (HD v1) c2 c3),v2,acc1)
        else
          let var = MAX (FST acc2) (FST acc3) in
-          (Seq c1 (If (HD v1) (Seq c2 (Move var (HD v2)))
-                              (Seq c3 (Move var (HD v3)))),
-           [var],(var+1,SND acc1))) /\
+         let (live,rest) = SND acc1 in
+           (Seq c1 (If (HD v1) (Seq c2 (Move var (HD v2)))
+                               (Seq c3 (Move var (HD v3)))),
+           [var],(var+1,insert var () live,rest))) /\
   (compile acc env tail [Let xs x2] =
      let (c1,vs,acc1) = compile acc env F xs in
      let (c2,v2,acc2) = compile acc1 (vs ++ env) tail [x2] in
